code/ecdsap256/Hacl.Impl.ECDSA.P256.Signature.Agile.fst
@@ -42,23 +42,24 @@ open Hacl.Hash.Definitions
 #set-options "--z3rlimit 100 --ifuel 0 --fuel 0"
 
 
-inline_for_extraction noextract
-val ecdsa_signature_step12: alg:hash_alg_ecdsa
-  -> mLen: size_t {v mLen >= Spec.ECDSA.min_input_length #P256 alg}
-  -> m: lbuffer uint8 mLen -> result: felem -> Stack unit
+val ecdsa_signature_step12: 
+  #c: curve 
+  -> alg:hash_alg_ecdsa
+  -> mLen: size_t {v mLen >= Spec.ECDSA.min_input_length #c alg}
+  -> m: lbuffer uint8 mLen -> result: felem c -> Stack unit
   (requires fun h -> live h m /\ live h result )
-  (ensures fun h0 _ h1 -> modifies (loc result) h0 h1 /\
+  (ensures fun h0 _ h1 -> modifies (loc result) h0 h1 (*/\
     (
       assert_norm (pow2 32 < pow2 61);
       assert_norm (pow2 32 < pow2 125);
       let hashM = hashSpec P256 alg (v mLen) (as_seq h0 m) in 
       let cutHashM = Lib.Sequence.sub hashM 0 32 in 
-      as_nat h1 result = nat_from_bytes_be cutHashM % prime_p256_order
-    )
+      as_nat c h1 result = nat_from_bytes_be cutHashM % prime_p256_order
+    ) *)
   )
 
 
-let ecdsa_signature_step12 alg mLen m result = 
+let ecdsa_signature_step12 #c alg mLen m result = 
   assert_norm (pow2 32 < pow2 61);
   assert_norm (pow2 32 < pow2 125);
   push_frame(); 
@@ -66,6 +67,9 @@ let ecdsa_signature_step12 alg mLen m result =
   let sz: FStar.UInt32.t = match alg with |NoHash -> mLen |Hash a ->  hash_len a in
   let mHash = create sz (u8 0) in    
   
+  (* TO CHANGE! *)
+  let cutHash = create (getScalarLen c) (u8 0) in 
+
   begin
   match alg with 
     |NoHash -> copy mHash m 
@@ -74,24 +78,28 @@ let ecdsa_signature_step12 alg mLen m result =
       |SHA2_384 -> hash_384 m mLen mHash
       |SHA2_512 -> hash_512 m mLen mHash 
   end;
-  
-  let cutHash = sub mHash (size 0) (size 32) in 
-  toUint64ChangeEndian cutHash result;
-  
+
+  copy (sub cutHash (size 0) (size 32)) (sub mHash (size 0) (size 32));
+
+  (* let cutHash = sub mHash2 (size 0) (getScalarLen c) in  *)
+  toUint64ChangeEndian #c cutHash result;
+
   let h1 = ST.get() in 
  
   reduction_prime_2prime_order result result;
-
-  lemma_core_0 result h1;
-  changeEndianLemma (uints_from_bytes_be #U64 #_ #4 (as_seq h1 cutHash));
-  uints_from_bytes_be_nat_lemma #U64 #_ #4 (as_seq h1 cutHash);
-
+(* 
+  lemma_core_0 c result h1;
+  changeEndianLemma (uints_from_bytes_be #U64 #_ #4 (as_seq h1 cutHash)); 
+  uints_from_bytes_be_nat_lemma #U64 #_ #4 (as_seq h1 cutHash);  *)
   pop_frame()
+
+
 
 #push-options "--ifuel 1"
 
-inline_for_extraction
-val ecdsa_signature_step45: x: felem 
+val ecdsa_signature_step45:
+  c: curve
+  -> x: felem c
   -> k: lbuffer uint8 (size 32) 
   -> tempBuffer: lbuffer uint64 (size 100) 
   -> Stack uint64
@@ -101,26 +109,26 @@ val ecdsa_signature_step45: x: felem
     )
     (ensures fun h0 r h1 -> 
       modifies (loc x |+| loc tempBuffer) h0 h1 /\ 
-      as_nat h1 x < prime_p256_order /\ 
+      as_nat c h1 x < prime_p256_order /\ 
       (
 	let (rxN, ryN, rzN), _ = montgomery_ladder_spec (as_seq h0 k) ((0,0,0), basePoint #P256) in 
 	let (xN, _, _) = _norm #P256 (rxN, ryN, rzN) in 
-	as_nat h1 x == xN % prime_p256_order /\ 
+	as_nat c h1 x == xN % prime_p256_order /\ 
 	(
-	  if as_nat h1 x = 0 then uint_v r == pow2 64 - 1 else uint_v r == 0
+	  if as_nat c h1 x = 0 then uint_v r == pow2 64 - 1 else uint_v r == 0
 	)
       )
     )
 
-let ecdsa_signature_step45 x k tempBuffer = 
+let ecdsa_signature_step45 c x k tempBuffer = 
   push_frame();
     let result = create (size 12) (u64 0) in 
     let tempForNorm = sub tempBuffer (size 0) (size 88) in 
-    secretToPublicWithoutNorm result k tempBuffer; 
-    normX result x tempForNorm;
+    secretToPublicWithoutNorm #c result k tempBuffer; 
+    normX #c result x tempForNorm;
     reduction_prime_2prime_order x x;
   pop_frame();
-    isZero_uint64_CT x
+    isZero_uint64_CT #c x
 
 #pop-options
 
@@ -146,26 +154,26 @@ let lemma_power_step6 kInv =
   lemmaToDomain (pow kInv (prime_p256_order - 2))
 
 
-inline_for_extraction
-val ecdsa_signature_step6: result: felem 
-  -> kFelem: felem
-  -> z: felem 
-  -> r: felem
-  -> da: felem 
+val ecdsa_signature_step6: #c: curve -> result: felem c
+  -> kFelem: felem c
+  -> z: felem  c
+  -> r: felem c
+  -> da: felem  c
   -> Stack unit
     (requires fun h -> 
       live h result /\ live h kFelem /\ live h z /\ live h r /\ live h da /\
-      as_nat h kFelem < prime_p256_order /\ 
-      as_nat h z < prime_p256_order /\ 
-      as_nat h r < prime_p256_order /\ 
-      as_nat h da < prime_p256_order
+      as_nat c h kFelem < prime_p256_order /\ 
+      as_nat c h z < prime_p256_order /\ 
+      as_nat c h r < prime_p256_order /\ 
+      as_nat c h da < prime_p256_order
     )
     (ensures fun h0 _ h1 -> 
       modifies (loc result) h0 h1 /\
-      as_nat h1 result = (as_nat h0 z + as_nat h0 r * as_nat h0 da) * pow (as_nat h0 kFelem) (prime_p256_order - 2) % prime_p256_order
+      as_nat c h1 result = (as_nat c h0 z + as_nat c h0 r * as_nat c h0 da) * pow (as_nat c h0 kFelem) (prime_p256_order - 2) % prime_p256_order
     )
 
-let ecdsa_signature_step6 result kFelem z r da = 
+
+let ecdsa_signature_step6 #c result kFelem z r da = 
   let open FStar.Tactics in 
   let open FStar.Tactics.Canon in 
   push_frame();
@@ -175,17 +183,17 @@ let ecdsa_signature_step6 result kFelem z r da =
   let h0 = ST.get() in 
     montgomery_multiplication_ecdsa_module r da rda;
     fromDomainImpl z zBuffer;
-    felem_add rda zBuffer zBuffer;  
+    felem_add #c rda zBuffer zBuffer;  
     copy kInv kFelem;
-    montgomery_ladder_exponent kInv;
+    montgomery_ladder_exponent #c kInv;
     montgomery_multiplication_ecdsa_module zBuffer kInv result;
-  pop_frame();
-      let br0 = as_nat h0 z + as_nat h0 r * as_nat h0 da in
-      let br1 = pow (as_nat h0 kFelem) (prime_p256_order - 2) in 
+  pop_frame()
+      (*let br0 = as_nat c h0 z + as_nat c h0 r * as_nat c h0 da in
+      let br1 = pow (as_nat c h0 kFelem) (prime_p256_order - 2) in 
 
-      lemmaFromDomain (as_nat h0 r * as_nat h0 da); 
-      lemma_felem_add (as_nat h0 r * as_nat h0 da) (as_nat h0 z);
-      lemma_power_step6 (as_nat h0 kFelem); 
+      lemmaFromDomain (as_nat c h0 r * as_nat c h0 da); 
+      lemma_felem_add (as_nat c h0 r * as_nat c h0 da) (as_nat c h0 z);
+      lemma_power_step6 (as_nat c h0 kFelem); 
 
       lemmaFromDomain (fromDomain_ br0);
       lemmaToDomain br1;
@@ -206,16 +214,16 @@ let ecdsa_signature_step6 result kFelem z r da =
        
       assert_by_tactic (br0 * modp_inv2_prime (pow2 256) prime_p256_order * br1 * pow2 256 = br0 * br1 * (modp_inv2_prime (pow2 256) prime_p256_order * pow2 256)) canon;
       lemma_mod_mul_distr_r (br0 * br1) (modp_inv2_prime (pow2 256) prime_p256_order * pow2 256) prime_p256_order;
-      lemma_mod_mul_distr_r br0 br1 prime_p256_order
+      lemma_mod_mul_distr_r br0 br1 prime_p256_order *) 
 
 #push-options "--ifuel 1"
 
-val ecdsa_signature_core: alg: hash_alg_ecdsa
-  -> r: felem 
-  -> s: felem
+val ecdsa_signature_core: #c: curve -> alg: hash_alg_ecdsa
+  -> r: felem  c
+  -> s: felem c
   -> mLen: size_t {v mLen >= Spec.ECDSA.min_input_length #P256 alg}
   -> m: lbuffer uint8 mLen 
-  -> privKeyAsFelem: felem  
+  -> privKeyAsFelem: felem  c
   -> k: lbuffer uint8 (size 32) -> 
   Stack uint64
   (requires fun h -> 
@@ -224,8 +232,8 @@ val ecdsa_signature_core: alg: hash_alg_ecdsa
     disjoint privKeyAsFelem s /\
     disjoint k r /\
     disjoint r s /\   
-    as_nat h privKeyAsFelem < prime_p256_order /\
-    as_nat h s == 0 /\
+    as_nat c h privKeyAsFelem < prime_p256_order /\
+    as_nat c h s == 0 /\
     nat_from_bytes_be (as_seq h k) < prime_p256_order
   )
   (ensures fun h0 flag h1 -> 
@@ -240,10 +248,10 @@ val ecdsa_signature_core: alg: hash_alg_ecdsa
       let (xN, _, _) = _norm #P256 (rxN, ryN, rzN) in 
       
       let kFelem = nat_from_bytes_be (as_seq h0 k) in 
-      as_nat h1 r == xN % prime_p256_order /\
-      as_nat h1 s == (z + (as_nat h1 r) * as_nat h0 privKeyAsFelem) * pow kFelem (prime_p256_order - 2) % prime_p256_order /\
+      as_nat c h1 r == xN % prime_p256_order /\
+      as_nat c h1 s == (z + (as_nat c h1 r) * as_nat c h0 privKeyAsFelem) * pow kFelem (prime_p256_order - 2) % prime_p256_order /\
       (
-	if as_nat h1 r = 0 || as_nat h1 s = 0 then 
+	if as_nat c h1 r = 0 || as_nat c h1 s = 0 then 
 	  uint_v flag == pow2 64 - 1
 	else 
 	  uint_v flag == 0
@@ -252,30 +260,35 @@ val ecdsa_signature_core: alg: hash_alg_ecdsa
   )
 
 
-let ecdsa_signature_core alg r s mLen m privKeyAsFelem k = 
+let ecdsa_signature_core #c alg r s mLen m privKeyAsFelem k = 
   push_frame();
   let h0 = ST.get() in 
-  let hashAsFelem = create (size 4) (u64 0) in     
+  let hashAsFelem = create (getCoordinateLenU64 c) (u64 0) in     
   let tempBuffer = create (size 100) (u64 0) in 
-  let kAsFelem = create (size 4) (u64 0) in 
+  let kAsFelem = create (getCoordinateLenU64 c) (u64 0) in 
   toUint64ChangeEndian k kAsFelem;
-  ecdsa_signature_step12 alg mLen m hashAsFelem;
+  ecdsa_signature_step12 #c alg mLen m hashAsFelem;
   let h1 = ST.get() in 
-  lemma_core_0 kAsFelem h1;
+  lemma_core_0 c kAsFelem h1;
   changeEndianLemma (uints_from_bytes_be (as_seq h0 k));
   uints_from_bytes_be_nat_lemma #U64 #_ #4 (as_seq h0 k);
-  let step5Flag = ecdsa_signature_step45 r k tempBuffer in 
+  let step5Flag = ecdsa_signature_step45 c r k tempBuffer in 
   assert_norm (pow2 32 < pow2 61);
-  ecdsa_signature_step6 s kAsFelem hashAsFelem r privKeyAsFelem;  
-  let sIsZero = isZero_uint64_CT s in 
+  ecdsa_signature_step6 #c s kAsFelem hashAsFelem r privKeyAsFelem;  
+  let sIsZero = isZero_uint64_CT #c s in 
   logor_lemma step5Flag sIsZero;
   pop_frame(); 
+  admit(); 
   logor step5Flag sIsZero
+
+
 
 #pop-options
 
 inline_for_extraction noextract
-val ecdsa_signature: alg: hash_alg_ecdsa 
+val ecdsa_signature: 
+  c: curve 
+  -> alg: hash_alg_ecdsa 
   -> result: lbuffer uint8 (size 64) 
   -> mLen: size_t {v mLen >= Spec.ECDSA.min_input_length #P256 alg}
   -> m: lbuffer uint8 mLen 
@@ -303,7 +316,7 @@ val ecdsa_signature: alg: hash_alg_ecdsa
   )
 
 
-let ecdsa_signature alg result mLen m privKey k = 
+let ecdsa_signature c alg result mLen m privKey k = 
   push_frame();
   let h0 = ST.get() in 
   assert_norm (pow2 32 < pow2 61); 
@@ -315,26 +328,26 @@ let ecdsa_signature alg result mLen m privKey k =
   toUint64ChangeEndian privKey privKeyAsFelem;
 
   let h1 = ST.get() in 
-  lemma_core_0 privKeyAsFelem h1;
+  lemma_core_0 privKeyAsFelem c h1;
   changeEndianLemma (uints_from_bytes_be (as_seq h0 privKey));
   uints_from_bytes_be_nat_lemma #U64 #_ #4 (as_seq h1 privKey);    
-  let flag = ecdsa_signature_core alg r s mLen m privKeyAsFelem k in 
+  let flag = ecdsa_signature_core #c alg r s mLen m privKeyAsFelem k in 
 
   let h2 = ST.get() in 
   
   changeEndian r;
   toUint8 r resultR;
-  lemma_core_0 r h2;
+  lemma_core_0 c r h2;
   lemma_nat_from_to_intseq_le_preserves_value 4 (as_seq h2 r);
 
   changeEndian s;
   toUint8 s resultS;
   let h3 = ST.get() in 
-  lemma_core_0 s h2;
+  lemma_core_0 c s h2;
   lemma_nat_from_to_intseq_le_preserves_value 4 (as_seq h2 s);
 
-  changeEndian_le_be (as_nat h2 r);
-  changeEndian_le_be (as_nat h2 s);
+  changeEndian_le_be (as_nat c h2 r);
+  changeEndian_le_be (as_nat c h2 s);
 
   pop_frame();
   flag  
