code/ecdsap256/Hacl.P256.fst
@@ -30,52 +30,52 @@ open Hacl.Impl.ECDSA.P256.Verification.Agile
 
 
 let ecdsa_sign_p256_sha2 result mLen m privKey k = 
-  ecdsa_signature (Hash SHA2_256) result mLen m privKey k
+  ecdsa_signature P256 (Hash SHA2_256) result mLen m privKey k
 
 let ecdsa_sign_p256_sha384 result mLen m privKey k = 
-  ecdsa_signature (Hash SHA2_384) result mLen m privKey k
+  ecdsa_signature P256 (Hash SHA2_384) result mLen m privKey k
 
 let ecdsa_sign_p256_sha512 result mLen m privKey k = 
-  ecdsa_signature (Hash SHA2_512) result mLen m privKey k
+  ecdsa_signature P256 (Hash SHA2_512) result mLen m privKey k
 
 let ecdsa_sign_p256_without_hash result mLen m privKey k = 
-  ecdsa_signature NoHash result mLen m privKey k
+  ecdsa_signature P256 NoHash result mLen m privKey k
 
 
 let ecdsa_verif_p256_sha2 mLen m pubKey r s = 
-  ecdsa_verification (Hash SHA2_256) pubKey r s mLen m
+  ecdsa_verification P256 (Hash SHA2_256) pubKey r s mLen m
 
 let ecdsa_verif_p256_sha384 mLen m pubKey r s = 
-  ecdsa_verification (Hash SHA2_384) pubKey r s mLen m
+  ecdsa_verification P256 (Hash SHA2_384) pubKey r s mLen m
 
 let ecdsa_verif_p256_sha512 mLen m pubKey r s = 
-  ecdsa_verification (Hash SHA2_512) pubKey r s mLen m
+  ecdsa_verification P256 (Hash SHA2_512) pubKey r s mLen m
 
 let ecdsa_verif_without_hash mLen m pubKey r s  =
-   ecdsa_verification NoHash pubKey r s mLen m
+   ecdsa_verification P256 NoHash pubKey r s mLen m
 
 
 let verify_q pubKey = 
-    Hacl.Impl.P256.Signature.Common.verifyQ pubKey
+    Hacl.Impl.P256.Signature.Common.verifyQ #P256 pubKey
 
 
 let decompression_not_compressed_form b result = 
-  Hacl.Impl.P256.Compression.decompressionNotCompressedForm b result
+  Hacl.Impl.P256.Compression.decompressionNotCompressedForm #P256 b result
 
 let decompression_compressed_form b result = 
-  Hacl.Impl.P256.Compression.decompressionCompressedForm b result
+  Hacl.Impl.P256.Compression.decompressionCompressedForm #P256 b result
 
 
 
 let compression_not_compressed_form b result = 
-  Hacl.Impl.P256.Compression.compressionNotCompressedForm b result
+  Hacl.Impl.P256.Compression.compressionNotCompressedForm #P256 b result
 
 let compression_compressed_form b result = 
-  Hacl.Impl.P256.Compression.compressionCompressedForm b result
+  Hacl.Impl.P256.Compression.compressionCompressedForm #P256 b result
 
  
 
-let reduction_8_32 x result = Hacl.Impl.ECDSA.Reduction.reduction_8_32 x result 
+let reduction_8_32 x result = Hacl.Impl.ECDSA.Reduction.reduction_8_32 #P256 x result 
 
 
 
